examples/dsls/core/Refl.Typing.Builtins.fsti
@@ -1,0 +1,19 @@
+module Refl.Typing.Builtins
+
+module R = FStar.Reflection
+module T = FStar.Tactics
+
+val subtyping_token (g:R.env) (t0 t1:R.typ) : Type0
+
+val equiv_token (g:R.env) (t0 t1:R.typ) : Type0
+
+val typing_token (g:R.env) (e:R.term) (t:R.typ) : Type0
+
+val check_subtyping (g:R.env) (t0 t1:R.typ)
+  : T.Tac (option (squash (subtyping_token g t0 t1)))
+
+val check_equiv (g:R.env) (t0 t1:R.typ)
+  : T.Tac (option (squash (equiv_token g t0 t1)))
+
+val tc_term (g:R.env) (e:R.term)
+  : T.Tac (option (t:R.typ{typing_token g e t}))
